

讲义习题5.6:1-6.

Denote ${}^\sigma L : (\alpha_1, \dots, \alpha_r) \mapsto T(\alpha_{\sigma(1)}, \dots, \alpha_{\sigma(r)})$.

5.6.1

Verify that $AL \in \Lambda^r(V) \forall L \in \mathcal{T}^r(V)$.

Proof: Suppose $\alpha_1 = \alpha_2$, then $\tau = (12)$ is odd, so

$$AL = \sum_{\sigma \in S_r} \text{sgn}(\sigma) {}^\sigma L = \sum_{\sigma \in A_r} \text{sgn}(\sigma) {}^\sigma L + \sum_{\sigma \in A_r} \text{sgn}(\sigma\tau) {}^{\sigma\tau} L.$$

Since $\alpha_1 = \alpha_2$, $\text{sgn}(\sigma\tau) {}^{\sigma\tau} L(\alpha_1, \dots, \alpha_n) = -\text{sgn}(\sigma) {}^\sigma L(\alpha_1, \dots, \alpha_n)$, so $AL(\alpha_1, \dots, \alpha_r) = 0$.

5.6.2

Prove that AL is skew-symmetric.

Proof: Suppose $\alpha_1 = \alpha_2$, then $\tau = (12)$ is odd, so

$$\begin{aligned} AL(\alpha_1, \alpha_2, \dots) &= \sum_{\sigma \in S_r} \text{sgn}(\sigma) ({}^\sigma L)(\alpha_1, \dots, \alpha_r) = \sum_{\sigma \in S_r} \text{sgn}(\sigma) ({}^\sigma L)(\alpha_2, \alpha_1, \dots, \alpha_r) \\ &= \sum_{\sigma \in S_r} \text{sgn}(\sigma) ({}^{\sigma\tau} L)(\alpha_1, \dots, \alpha_r) = -AL(\alpha_1, \dots, \alpha_r). \end{aligned}$$

5.6.3

Prove that for $L \in \Lambda^r(V)$, $M \in \Lambda^s(V)$, $N \in \Lambda^t(V)$, then $(s+t)!A(A(L \otimes M) \otimes N) = (r+s)!A(L \otimes A(M \otimes N))$.

Proof:

$$\begin{aligned} A(A(L \otimes M) \otimes N) &= \sum_{\sigma \in S_{r+s+t}} \text{sgn}(\sigma) {}^\sigma (A(L \otimes M) \otimes N) = \sum_{\sigma \in S_{r+s+t}} \sum_{\tau \in S_{r+s}} \text{sgn}(\sigma) \text{sgn}(\tau) {}^{\sigma\tau} (L \otimes M) \otimes N \\ &= \sum_{\tau \in S_{r+s}} \sum_{\sigma \in S_{r+s+t}} \text{sgn}(\sigma\tau) {}^{\sigma\tau} (L \otimes M \otimes N) \\ &= \sum_{\tau \in S_{r+s}} \sum_{\sigma \in S_{r+s+t}} \text{sgn}(\sigma) {}^\sigma (L \otimes M \otimes N) = (r+s)! \sum_{\sigma \in S_{r+s+t}} \text{sgn}(\sigma) {}^\sigma (L \otimes M \otimes N). \end{aligned}$$

Likewise we obtain $(s+t)!A(A(L \otimes M) \otimes N) = (r+s)!A(L \otimes A(M \otimes N))$.

5.6.4

Suppose $\text{char } F = 0$. Verify that $L \wedge M = \frac{1}{(r+s)!} A(L \otimes M)$ and $L \wedge_1 M = \frac{1}{r!s!} A(L \otimes M)$ are both commutative.

Proof: By 5.6.3

$$\begin{aligned} (L \wedge M) \wedge N &= \left(\frac{1}{(r+s)!} A(L \otimes M) \right) \wedge N = \frac{1}{(r+s)!(r+s+t)!} A(A(L \otimes M) \otimes N) \\ &= \frac{1}{(s+t)!(r+s+t)!} A(L \otimes A(M \otimes N)) = L \wedge (M \wedge N). \end{aligned}$$

And likewise $(L \wedge_1 M) \wedge_1 N = L \wedge_1 (M \wedge_1 N)$.

5.6.5

Suppose $\text{char } F = 0$ verify that for $L \in \Lambda^r(V)$, $M \in \Lambda^s(V)$,

$$A\left(\frac{L}{r!} \otimes \frac{M}{s!}\right) = \sum_{\sigma \in Sh(r,s)} \text{sgn}(\sigma)^\sigma (L \otimes M).$$

Proof:

$$\begin{aligned} A(L \otimes M) &= \sum_{\sigma \in S_{r+s}} \text{sgn}(\sigma)^\sigma (L \otimes M) = \sum_{\sigma \in Sh(r,s)} \sum_{\tau \in S_r, \rho \in S_s} \text{sgn}(\sigma \circ (\tau \times \rho))^\sigma (\tau L \otimes^\rho M) \\ &= r!s! \sum_{\sigma \in Sh(r,s)} \text{sgn}(\sigma) (L \otimes M) \end{aligned}$$

5.6.6

Suppose r is odd, $L \in \Lambda^r(V)$. Prove that $L \wedge L = 0$.

Proof: Take $\tau = (1, r+1)(2, r+2) \cdots (r, 2r)$, then $\text{sgn}(\tau) = -1$ and ${}^\tau(L \otimes L) = L \otimes L$ so

$$L \wedge L = \frac{1}{(2r)!} \sum_{\sigma \in S_{2r}} \text{sgn}(\sigma)^\sigma (L \otimes L) = \frac{1}{(2r)!} \sum_{\sigma \in A_{2r}} \text{sgn}(\sigma)^\sigma (L \otimes L) + \text{sgn}(\sigma\tau)^{\sigma\tau} (L \otimes L) = 0.$$